inv_ack_standalone.v
@@ -1,6 +1,10 @@
 Require Import Omega.
 Require Import Program.Basics.
+Require Import BinNat.
 
+(* ********** COUNTDOWN AND INVERSE ACKERMANN ON NAT ********** *)
+
+(* Countdown worker function *)
 Fixpoint countdown_worker (f : nat -> nat) (a n k : nat) : nat :=
   match k with
   | 0    => 0
@@ -8,8 +12,10 @@ Fixpoint countdown_worker (f : nat -> nat) (a n k : nat) : nat :=
               S (countdown_worker f a (f n) k')
   end.
 
+(* Countdown *)
 Definition countdown_to f a n := countdown_worker f a n n.
 
+(* Inverse Ackermann worker function *)
 Fixpoint inv_ack_worker (f : nat -> nat) (n k b : nat) : nat :=
   match b with
   | 0    => k
@@ -20,8 +26,58 @@ Fixpoint inv_ack_worker (f : nat -> nat) (n k b : nat) : nat :=
             end
   end.
 
+(* Inverse Ackermann function *)
+(* Definition by hard-coding up to the second bin_alpha level, runtime O(n) *)
 Definition inv_ack_linear n :=
   match n with
   | 0 | 1 => 0
   | _     => let f := (fun x => x - 2) in inv_ack_worker f (f n) 1 (n - 1)
   end.
+
+
+(* ********** COUNTDOWN AND INVERSE ACKERMANN ON N (BINARY) ********** *)
+
+Open Scope N_scope.
+
+(* Supporting function - Use to compute the budget for bin_cdn_wkr and inv_ack_wrk
+   Returns length of the binary representation in type "nat" *)
+Definition nat_size (n : N) : nat :=
+  match n with
+  | 0 => 0%nat
+  | Npos p => let fix nat_pos_size (x : positive) : nat :=
+                  match x with
+                  | xH => 1%nat
+                  | xI y | xO y => S (nat_pos_size y) end
+                  in nat_pos_size p
+  end.
+
+(* Countdown worker function *)
+Fixpoint bin_cdn_wkr (f : N -> N) (a n : N) (b : nat) : N :=
+  match b with
+  | O    => 0
+  | S b' => if (n <=? a) then 0
+             else 1 + bin_cdn_wkr f a (f n) b'
+  end.
+
+(* Countdown *)
+Definition bin_countdown_to (f : N -> N) (a n : N) : N
+  := bin_cdn_wkr f a n (nat_size (n - a)).
+
+(* Inverse Ackermann worker function *)
+Fixpoint bin_inv_ack_worker (f : N -> N) (n k : N) (bud : nat) : N :=
+  match bud with
+  | 0%nat  => k
+  | S bud' =>
+    if n <=? k then k
+      else let g := (bin_countdown_to f 1) in
+      bin_inv_ack_worker (compose g f) (g n) (N.succ k) bud'
+  end.
+
+(* Inverse Ackermann function *)
+(* Definition by hard-coding up to the fourth bin_alpha level, runtime O(log n) *)
+Definition bin_inv_ack n :=
+  if (n <=? 1) then 0
+  else if (n <=? 3) then 1
+  else if (n <=? 7) then 2
+  else let f := (fun x => N.log2 (x + 2) - 2) in
+        bin_inv_ack_worker f (f n) 3 (nat_size n).
